src/program_proof/memkv/memkv_marshal_put_proof.v
@@ -24,7 +24,7 @@ Record PutReplyC := mkPutReplyC {
 Definition own_PutRequest args_ptr val_sl args : iProp Σ :=
   "HKey" ∷ args_ptr ↦[PutRequest :: "Key"] #args.(PR_Key) ∗
   "HValue" ∷ args_ptr ↦[PutRequest :: "Value"] (slice_val val_sl) ∗
-  "#HValue_sl" ∷ readonly (typed_slice.own_slice_small val_sl byteT 1 args.(PR_Value))
+  "#HValue_sl" ∷ readonly (typed_slice.own_slice_small val_sl byteT (DfracOwn 1) args.(PR_Value))
 .
 
 Definition own_PutReply reply_ptr rep : iProp Σ :=
@@ -44,7 +44,7 @@ Lemma wp_EncodePutRequest args_ptr val_sl args :
     EncodePutRequest #args_ptr
   {{{
        (reqData:list u8) req_sl, RET (slice_val req_sl); ⌜has_encoding_PutRequest reqData args⌝ ∗
-                                               typed_slice.own_slice req_sl byteT 1%Qp reqData ∗
+                                               typed_slice.own_slice req_sl byteT (DfracOwn 1) reqData ∗
                                                own_PutRequest args_ptr val_sl args
   }}}.
 Proof.
@@ -98,7 +98,7 @@ Qed.
 Lemma wp_DecodePutRequest req_sl reqData args :
   {{{
        ⌜has_encoding_PutRequest reqData args⌝ ∗
-       typed_slice.own_slice_small req_sl byteT 1%Qp reqData
+       typed_slice.own_slice_small req_sl byteT (DfracOwn 1) reqData
   }}}
     DecodePutRequest (slice_val req_sl)
   {{{
@@ -124,7 +124,7 @@ Proof.
 
   wp_apply (wp_Dec__GetInt with "[$Hdec]").
   iIntros "Hdec".
-  wp_apply (wp_Dec__GetBytes_ro with "[$Hdec]"); first done.
+  wp_apply (wp_Dec__GetBytes with "[$Hdec]"); first done.
   iIntros (??) "[Hsl Hdec]".
   wp_storeField.
 
@@ -141,7 +141,7 @@ Lemma wp_EncodePutReply rep_ptr rep :
     EncodePutReply #rep_ptr
   {{{
        repData rep_sl , RET (slice_val rep_sl);
-       typed_slice.own_slice rep_sl byteT 1%Qp repData ∗
+       typed_slice.own_slice rep_sl byteT (DfracOwn 1) repData ∗
        ⌜has_encoding_PutReply repData rep ⌝
   }}}.
 Proof.
@@ -173,7 +173,7 @@ Qed.
 
 Lemma wp_DecodePutReply rep rep_sl repData :
   {{{
-       typed_slice.own_slice_small rep_sl byteT 1%Qp repData ∗
+       typed_slice.own_slice_small rep_sl byteT (DfracOwn 1) repData ∗
        ⌜has_encoding_PutReply repData rep ⌝
   }}}
     DecodePutReply (slice_val rep_sl)
